theories/ml_toy_lang/melocoton/primitive_laws.v
@@ -9,12 +9,16 @@ From melocoton.language Require Export weakestpre lifting.
 From melocoton.ml_toy_lang Require Export melocoton.class_instances.
 From melocoton.ml_toy_lang Require Import melocoton.tactics notation.
 From iris.prelude Require Import options.
+From melocoton Require Import monotone.
+Search "view" "GS".
 
 Class heapGS_ML Σ := HeapGS_ML {
   heapGS_gen_heapGS :> gen_heapGS loc (option (list val)) Σ;
   heapGS_inv_heapGS :> inv_heapGS loc (option (list val)) Σ;
   heapGS_step_name : gname;
   heapGS_step_cnt : mono_natG Σ;
+  heapGS_store_domain : inG Σ (viewUR (@auth_view_rel (@monotoneUR (leibnizO (gset loc)) subseteq)));
+  heapGS_store_domain_name : gname
 }.
 Local Existing Instance heapGS_step_cnt.
 
@@ -55,14 +59,207 @@ Section steps.
 
 End steps.
 
+Section DomAuth.
+  Context `{!heapGS_ML Σ}.
+
+  Definition dom_auth (σ : gmap loc (option (list val))) : iProp Σ := 
+    (@own _ _ heapGS_store_domain heapGS_store_domain_name (@auth_auth (@monotoneUR (leibnizO (gset loc)) subseteq) (DfracOwn (pos_to_Qp 1)) (principal subseteq (dom σ))))%I.
+
+  Definition dom_part (σ : gset loc) : iProp Σ := 
+    (@own _ _ heapGS_store_domain heapGS_store_domain_name (@auth_frag (@monotoneUR (leibnizO (gset loc)) subseteq) (principal subseteq (σ))))%I.
+
+  Global Instance subseteq_preorder : PreOrder (subseteq : gset loc -> gset loc -> Prop).
+  Proof. repeat split; eauto. intros a b c; set_solver. Qed.
+
+  Global Instance dom_part_timeless σ : Timeless (dom_part σ).
+  Proof. apply own_timeless. apply _. Qed.
+
+  Lemma dom_auth_dom σ1 σ2 : dom σ1 = dom σ2 -> dom_auth σ1 -∗ dom_auth σ2.
+  Proof. iIntros (Hdom) "H1". unfold dom_auth; rewrite Hdom; done. Qed.
+
+  Lemma dom_auth_part_valid σ σsub : dom_auth σ -∗ dom_part σsub -∗ ⌜σsub ⊆ dom σ⌝.
+  Proof.
+    iIntros "H1 H2".
+    iPoseProof (own_valid_2 with "H1 H2") as "%Hvalid".
+    iPureIntro.
+    apply auth_both_valid in Hvalid.
+    destruct Hvalid as (Hv1 & _).
+    specialize (Hv1 0). cbn in Hv1.
+    by eapply (@principal_includedN (leibnizO (gset loc)) _ subseteq_preorder).
+  Qed.
+
+  Lemma dom_auth_extend σ σnew : dom_auth σ -∗ ⌜dom σ ⊆ dom σnew⌝ ==∗ dom_auth σnew.
+  Proof.
+    iIntros "H1 %H2".
+    iMod (own_update with "H1") as "$"; last done. 
+    eapply auth_update_auth.
+    eapply monotone_local_update_grow. done.
+  Qed.
+
+  Lemma dom_auth_get σ σfrag : dom_auth σ -∗ ⌜σfrag ⊆ dom σ⌝ ==∗ dom_auth σ ∗ dom_part σfrag.
+  Proof.
+    iIntros "H1 %H2". 
+    iMod (own_update with "H1") as "(H1 & H2)".
+    1: eapply monotone_update; [done | apply H2].
+    iModIntro. iFrame.
+  Qed.
+
+End DomAuth.
+
+Section SafeValues.
+  Context `{!heapGS_ML Σ}.
+
+  Fixpoint val_safe_on_heap (σ : state) (v:val) : Prop := match v with
+      LitV (LitInt _) => True
+    | LitV (LitBool _) => True
+    | LitV (LitUnit) => True
+    | LitV (LitPoison) => False
+    | LitV (LitLoc l) => l ∈ dom σ
+    | PairV v1 v2 => val_safe_on_heap σ v1 ∧ val_safe_on_heap σ v2
+    | InjLV vl => val_safe_on_heap σ vl
+    | InjRV vr => val_safe_on_heap σ vr
+    | RecV f x e => True end.
+
+  Fixpoint val_safe (v : val) : iProp Σ := match v with
+      LitV (LitInt _) => True
+    | LitV (LitBool _) => True
+    | LitV (LitUnit) => True
+    | LitV (LitPoison) => False
+    | LitV (LitLoc l) => dom_part {[ l ]}
+    | PairV v1 v2 => val_safe v1 ∗ val_safe v2
+    | InjLV vl => val_safe vl
+    | InjRV vr => val_safe vr
+    | RecV f x e => True end.
+
+  Global Instance safe_persistent v : Persistent (val_safe v).
+  Proof.
+   induction v as [[z|b| | |l]|v1 IH1 v2|vl IH|vr IH|]; apply _.
+  Qed.
+
+  Global Instance safe_timeless v : Timeless (val_safe v).
+  Proof.
+   induction v as [[z|b| | |l]|v1 IH1 v2|vl IH|vr IH|]; apply _.
+  Qed.
+
+
+  Lemma val_safe_to_ghost_state σ v:
+     ⌜val_safe_on_heap σ v⌝
+   -∗ dom_auth σ
+  ==∗ dom_auth σ ∗ val_safe v.
+  Proof.
+    iIntros "%Hd Hσ"; iInduction (v) as [[z|b| | |l]|v1 v2|vl|vr|] "IH"; cbn in Hd; cbn; try (iModIntro; iFrame; done).
+    + apply singleton_subseteq_l in Hd. iApply (dom_auth_get with "Hσ []"). done.
+    + destruct Hd. iMod ("IH" with "[] Hσ") as "(Hσ & H1)"; first done.
+      iMod ("IH1" with "[] Hσ") as "(Hσ & H2)"; first done. iModIntro; iFrame.
+    + iMod ("IH" with "[] Hσ") as "(Hσ & H1)"; first done. iModIntro; iFrame.
+    + iMod ("IH" with "[] Hσ") as "(Hσ & H1)"; first done. iModIntro; iFrame.
+  Qed.
+
+  Lemma val_safe_of_ghost_state σ v:
+      dom_auth σ
+   -∗ val_safe v
+   -∗⌜val_safe_on_heap σ v⌝.
+  Proof.
+    iIntros "Hσ #Hs"; iInduction (v) as [[z|b| | |l]|? ?|vl|vr|] "IH"; cbn; try done.
+    + iPoseProof (dom_auth_part_valid with "Hσ Hs") as "%HH". iPureIntro. set_solver.
+    + iDestruct "Hs" as "(Hs1 & Hs2)".
+      iPoseProof ("IH" with "Hs1 Hσ") as "%H1".
+      iPoseProof ("IH1" with "Hs2 Hσ") as "%H2". iPureIntro; done.
+    + iPoseProof ("IH" with "Hs Hσ") as "%H1"; done.
+    + iPoseProof ("IH" with "Hs Hσ") as "%H1"; done.
+  Qed.
+
+  Definition val_arr_safe_on_heap (σ : state) (vs:list val) : Prop := Forall (val_safe_on_heap σ) vs.
+  Definition val_arr_safe (vs:list val) : iProp Σ := [∗ list] v ∈ vs, val_safe v.
+
+
+  Global Instance arr_safe_timeless v : Timeless (val_arr_safe v).
+  Proof.
+    apply _.
+  Qed.
+
+  Lemma val_arr_safe_to_ghost_state σ vs:
+     ⌜val_arr_safe_on_heap σ vs⌝
+   -∗ dom_auth σ
+  ==∗ dom_auth σ ∗ val_arr_safe vs.
+  Proof.
+    iInduction vs as [|v vs] "IH"; iIntros "%Hv Hσ".
+    + iModIntro. cbn. iPoseProof (bi.emp_sep_1 with "Hσ") as "($&$)".
+    + apply Forall_cons_1 in Hv. destruct Hv as (Hv & Hvs). 
+      iMod ("IH" with "[] Hσ") as "(Hσ & Hvs)"; first done. 
+      iMod (val_safe_to_ghost_state with "[] Hσ") as "(Hσ & Hv)"; first done.
+      iModIntro; iFrame.
+  Qed.
+
+  Lemma val_arr_safe_of_ghost_state σ vs:
+      dom_auth σ
+   -∗ val_arr_safe vs
+   -∗⌜val_arr_safe_on_heap σ vs⌝.
+  Proof.
+    iInduction vs as [|v vs] "IH"; iIntros "Hσ Hv".
+    + iPureIntro; cbn. econstructor.
+    + iDestruct "Hv" as "(Hv & Hvs)".
+      iPoseProof ("IH" with "Hσ Hvs") as "%Hvs".
+      iPoseProof (val_safe_of_ghost_state with "Hσ Hv") as "%Hv".
+      iPureIntro; by econstructor.
+  Qed.
+
+  Definition heap_part_safe_on_heap (σ : state) (σpart : gmap loc (option (list val))) : Prop := 
+   map_Forall (fun x y => match y with Some vs => val_arr_safe_on_heap σ vs | _ => True end) σpart.
+  Definition heap_safe (σ : gmap loc (option (list val))) : iProp Σ := 
+    [∗ map] k↦v ∈ σ, match v with Some vs => val_arr_safe vs | _ => True end.
+
+
+  Global Instance heap_safe_timeless v : Timeless (val_arr_safe v).
+  Proof.
+    apply _.
+  Qed.
+
+  Lemma heap_safe_to_ghost_state σ σ1:
+     ⌜heap_part_safe_on_heap σ σ1⌝
+   -∗ dom_auth σ
+  ==∗ dom_auth σ ∗ heap_safe σ1.
+  Proof.
+    induction σ1 using map_ind; iIntros "%Hsafe Hσ".
+    + iModIntro. cbn. iPoseProof (bi.emp_sep_1 with "Hσ") as "(Hemp&$)".
+      by iApply big_sepM_empty.
+    + iMod (IHσ1 with "[] Hσ") as "(Hσ & Hvs)". 1: iPureIntro; eapply map_Forall_insert_1_2; done.
+      destruct x as [vs|].
+      * iMod (val_arr_safe_to_ghost_state with "[] Hσ") as "(Hσ & Hv)". 1: eapply map_Forall_insert_1_1 in Hsafe; done. 
+        iModIntro. iFrame. unfold heap_safe. iApply big_sepM_insert; first done. iFrame.
+      * iModIntro. iFrame. unfold heap_safe. iApply big_sepM_insert; first done. iFrame.
+  Qed.
+
+  Lemma heap_safe_of_ghost_state σ σ1:
+      dom_auth σ
+   -∗ heap_safe σ1
+   -∗⌜heap_part_safe_on_heap σ σ1⌝.
+  Proof.
+    induction σ1 using map_ind; iIntros "Hσ Hv".
+    + iPureIntro; cbn. eapply map_Forall_empty.
+    + iPoseProof (big_sepM_insert) as "(Ha & _)"; first done.
+      iPoseProof ("Ha" with "Hv") as "(Hvs & Hh)"; iClear "Ha".
+      iPoseProof (IHσ1 with "Hσ Hh") as "%Hh".
+      destruct x as [vs|].
+      * iPoseProof (val_arr_safe_of_ghost_state with "Hσ Hvs") as "%Hvs".
+        iPureIntro. apply map_Forall_insert; done.
+      * iPureIntro. apply map_Forall_insert; done.
+  Qed.
+
+End SafeValues.
+
+
 
 Global Program Instance heapGS_langGS_ML `{heapGS_ML Σ}
       : langGS val ML_lang Σ := {
   state_interp σ step_cnt :=
-    (gen_heap_interp σ ∗ steps_auth step_cnt)%I
+    ( gen_heap_interp σ
+    ∗ steps_auth step_cnt
+    ∗ dom_auth σ
+    ∗ heap_safe σ)%I
 }.
 Next Obligation.
-  iIntros (???? σ ns E)  "/= ($ & H)".
+  iIntros (???? σ ns E)  "/= ($ & H & $)".
   by iMod (steps_auth_update_S with "H") as "$".
 Qed.
 
@@ -134,7 +331,7 @@ Proof.
   (** TODO: We should try to use a generic lifting lemma (and avoid [wp_unfold])
   here, since this breaks the WP abstraction. *)
   rewrite !wp_unfold /wp_pre /=. iIntros (Heq) "Hwp".
-  iIntros (σ1 ns) "(Hσ & Hsteps)".
+  iIntros (σ1 ns) "(Hσ & Hsteps & Hdom)".
   iDestruct (steps_lb_get with "Hsteps") as "#Hlb".
   iDestruct (steps_lb_le _ 0 with "Hlb") as "Hlb0"; [lia|].
   iSpecialize ("Hwp" with "Hlb0"). iApply ("Hwp" $! σ1 ns). iFrame.
@@ -149,20 +346,20 @@ Proof.
   (** TODO: We should try to use a generic lifting lemma (and avoid [wp_unfold])
   here, since this breaks the WP abstraction. *)
   rewrite !wp_unfold /wp_pre /=. iIntros (Heq) "Hlb Hwp".
-  iIntros (σ1 ns) "(Hσ & Hsteps)".
+  iIntros (σ1 ns) "(Hσ & Hsteps & Hdom & Hsafe)".
   iDestruct (steps_lb_valid with "Hsteps Hlb") as %?.
-  iMod ("Hwp" $! σ1 ns with "[$Hσ $Hsteps]") 
+  iMod ("Hwp" $! σ1 ns with "[$Hσ $Hsteps $Hdom $Hsafe]") 
       as "[(%v & -> & Hσ & Hv)|[(%s0 & %vv & %K & -> & Hprog & Hwp)|(%Hred & Hwp)]]".
   - cbn in Heq. apply TCEq_eq in Heq. congruence.
   - iModIntro. iRight. iLeft. iExists s0, vv, K. iFrame. iSplitR; first done.
-    iMod "Hwp" as "(%Ξ & (Hσ & Hsteps) & HΞ & Hwp)". iModIntro. 
+    iMod "Hwp" as "(%Ξ & (Hσ & Hsteps & Hdom) & HΞ & Hwp)". iModIntro. 
     iDestruct (steps_lb_get with "Hsteps") as "#HlbS".
     iExists Ξ. iFrame. iNext.
     iIntros (r) "Hr". iSpecialize ("Hwp" $! r with "Hr").
     iApply (wp_wand with "Hwp"). iIntros (v) "Hv". by iApply "Hv".
   - iModIntro. iRight. iRight. iSplitR; first done.
     iIntros (e2 σ2 Hstep). iMod ("Hwp" with "[//]") as "Hwp".
-    iIntros "!> !>". iMod "Hwp" as "((Hσ & Hsteps) & Hwp)". iIntros "!>".
+    iIntros "!> !>". iMod "Hwp" as "((Hσ & Hsteps & Hdom & Hsafe) & Hwp)". iIntros "!>".
     iDestruct (steps_lb_get with "Hsteps") as "#HlbS".
     iDestruct (steps_lb_le _ (S n) with "HlbS") as "#HlbS'"; [lia|].
     iFrame.
@@ -203,7 +400,7 @@ Lemma mapsto_combine l dq1 dq2 v1 v2 :
 Proof.
   iIntros "Hl1 Hl2". iDestruct (mapsto_combine with "Hl1 Hl2") as "[$ Heq]".
   by iDestruct "Heq" as %[= ->].
-Qed.
+Qed. 
 
 Lemma mapsto_frac_ne l1 l2 dq1 dq2 v1 v2 :
   ¬ ✓(dq1 ⋅ dq2) → l1 ↦M{dq1} v1 -∗ l2 ↦M{dq2} v2 -∗ ⌜l1 ≠ l2⌝.
@@ -267,55 +464,65 @@ Qed.
 
 Lemma wp_allocN pe E v n :
   (0 ≤ n)%Z →
-  {{{ True }}} AllocN (Val $ LitV $ LitInt n) (Val v) @ pe; E
-  {{{ l, RET LitV (LitLoc l); l ↦∗ (replicate (Z.to_nat n) v) ∗ meta_token l ⊤ }}}.
+  {{{ ▷ val_safe v }}} AllocN (Val $ LitV $ LitInt n) (Val v) @ pe; E
+  {{{ l, RET LitV (LitLoc l); l ↦∗ (replicate (Z.to_nat n) v) ∗ meta_token l ⊤ ∗ val_safe (#l) }}}.
 Proof.
-  iIntros (Hn Φ) "_ HΦ". iApply wp_lift_atomic_head_step; first done.
-  iIntros (σ1 ns) "(Hσ & Hsteps)". iModIntro. iSplit; first (destruct n; eauto with lia head_step).
+  iIntros (Hn Φ) ">#Hsafe HΦ". iApply wp_lift_atomic_head_step; first done.
+  iIntros (σ1 ns) "(Hσ & Hsteps & Hdom & Hheap)". iModIntro. iSplit; first (destruct n; eauto with lia head_step).
   iIntros (v2 σ2 Hstep). inv_head_step. iModIntro.
   iMod (gen_heap_alloc _ l (Some (replicate (Z.to_nat n) v)) with "Hσ") as "(Hσ & Hl & Hm)".
   { by apply not_elem_of_dom. }
   iMod (steps_auth_update_S with "Hsteps") as "Hsteps".
-  iModIntro. iFrame. iApply "HΦ". by iFrame.
+  iMod (dom_auth_extend with "Hdom []") as "Hdom"; last first.
+  1: iMod (dom_auth_get _ {[l]} with "Hdom []") as "(Hdom & #Hpart)"; first last.
+  1: iFrame "Hdom".
+  3: iPureIntro; rewrite dom_insert_L; set_solver.
+  2: iPureIntro; rewrite dom_insert_L; set_solver.
+  iModIntro. iFrame. iSplitL "Hsafe Hheap"; last iApply "HΦ"; iFrame; last done.
+  iApply big_sepM_insert. 1: by eapply not_elem_of_dom. iFrame.
+  iApply big_sepL_forall. iIntros (k x Hkx). apply lookup_replicate in Hkx. destruct Hkx; subst; done.
 Qed.
 
 Lemma wp_alloc pe E v :
-  {{{ True }}} Alloc (Val v) @ pe; E
-  {{{ l, RET LitV (LitLoc l); l ↦M v ∗ meta_token l ⊤ }}}.
+  {{{ ▷ val_safe v }}} Alloc (Val v) @ pe; E
+  {{{ l, RET LitV (LitLoc l); l ↦M v ∗ meta_token l ⊤ ∗ val_safe (#l) }}}.
 Proof.
-  iIntros (HΦ) "_ HΦ". by iApply wp_allocN.
+  iIntros (HΦ) ">#Hsafe HΦ". by iApply wp_allocN.
 Qed.
 
 Lemma wp_loadN pe E l i dq vs v :
   (0 ≤ i)%Z →
   vs !! Z.to_nat i = Some v →
   {{{ ▷ l ↦∗{dq} vs }}} LoadN (Val $ LitV $ LitLoc l) (Val $ LitV $ LitInt i) @ pe; E
-  {{{ RET v; l ↦∗{dq} vs }}}.
+  {{{ RET v; l ↦∗{dq} vs ∗ val_arr_safe vs }}}.
 Proof.
   iIntros (Hi Hv Φ) ">Hl HΦ". iApply wp_lift_atomic_head_step; first done.
-  iIntros (σ1 ns) "(Hσ & Hsteps) !>". iDestruct (gen_heap_valid with "Hσ Hl") as %?.
+  iIntros (σ1 ns) "(Hσ & Hsteps & Hdom & #Hsafe) !>". iDestruct (gen_heap_valid with "Hσ Hl") as %?.
   assert (σ1 !! l.[i] = Some v).
   { rewrite store_lookup_eq. case_bool_decide; [|done]. by simplify_map_eq/=. }
   iSplit; first by eauto with head_step.
   iIntros (v2 σ2 Hstep); inv_head_step. iModIntro.
-  iMod (steps_auth_update_S with "Hsteps") as "Hsteps". iFrame.
-  by iApply "HΦ".
+  iMod (steps_auth_update_S with "Hsteps") as "Hsteps". iModIntro. iFrame. iFrame "Hsafe".
+  iApply "HΦ". iFrame.
+  iPoseProof (big_sepM_lookup with "Hsafe") as "HH"; first done. iApply "HH".
 Qed.
 
 Lemma wp_load pe E l dq v :
   {{{ ▷ l ↦M{dq} v }}} Load (Val $ LitV $ LitLoc l) @ pe; E
-  {{{ RET v; l ↦M{dq} v }}}.
+  {{{ RET v; l ↦M{dq} v ∗ val_safe v }}}.
 Proof.
-  iIntros (Φ) ">Hl HΦ". by iApply (wp_loadN with "Hl").
+  iIntros (Φ) ">Hl HΦ". iApply (wp_loadN with "Hl"); try done.
+  iIntros "!> (H1 & #H2)". iApply "HΦ"; iFrame.
+  iPoseProof big_sepL_singleton as "[HL HR]".  unfold val_arr_safe. iPoseProof ("HL" with "H2") as "$".
 Qed.
 
 Lemma wp_storeN pe E l i vs w :
   (0 ≤ i < length vs)%Z →
-  {{{ ▷ l ↦∗ vs }}} StoreN (Val $ LitV $ LitLoc l) (Val $ LitV $ LitInt i) (Val w) @ pe; E
+  {{{ ▷ l ↦∗ vs ∗ ▷ val_safe w}}} StoreN (Val $ LitV $ LitLoc l) (Val $ LitV $ LitInt i) (Val w) @ pe; E
   {{{ RET LitV LitUnit; l ↦∗ <[ Z.to_nat i := w ]> vs }}}.
 Proof.
-  iIntros (Hi Φ) ">Hl HΦ". iApply wp_lift_atomic_head_step; first done.
-  iIntros (σ1 ns) "(Hσ & Hsteps) !>". iDestruct (gen_heap_valid with "Hσ Hl") as %?.
+  iIntros (Hi Φ) "(>Hl & >#Hsafe) HΦ". iApply wp_lift_atomic_head_step; first done.
+  iIntros (σ1 ns) "(Hσ & Hsteps & Hdom & #Hheap) !>". iDestruct (gen_heap_valid with "Hσ Hl") as %?.
   assert (is_Some (σ1 !! l.[i])) as [? ?].
   { rewrite store_lookup_eq. case_bool_decide; [|lia]. simplify_map_eq.
     apply lookup_lt_is_Some. lia. }
@@ -324,11 +531,17 @@ Proof.
   iMod (steps_auth_update_S with "Hsteps") as "Hsteps".
   iMod (gen_heap_update with "Hσ Hl") as "[Hσ Hl]".
   rewrite (store_insert_offset _ _ _ vs); auto; [].
-  iFrame "Hσ Hsteps". by iApply "HΦ".
+  iModIntro. iFrame "Hσ Hsteps". iSplitL "Hdom"; last by iApply "HΦ".
+  iSplitL.
+  + iApply dom_auth_dom; last done. rewrite dom_insert_L. eapply elem_of_dom_2 in H; set_solver.
+  + iApply big_sepM_insert_override_2; try done. iIntros "#Hvs".
+    iPoseProof (big_sepL_insert_acc with "Hvs") as "(_ & Hvs2)"; last by iApply "Hvs2".
+    rewrite store_lookup_eq in H0. rewrite bool_decide_decide in H0. destruct (decide); try lia.
+    rewrite H in H0. cbn in H0. done.
 Qed.
 
 Lemma wp_store pe E l v w :
-  {{{ ▷ l ↦M v }}} Store (Val $ LitV $ LitLoc l) (Val w) @ pe; E
+  {{{ ▷ l ↦M v  ∗ ▷ val_safe w}}} Store (Val $ LitV $ LitLoc l) (Val w) @ pe; E
   {{{ RET LitV LitUnit; l ↦M w }}}.
 Proof.
   iIntros (Φ) "Hl HΦ". by iApply (wp_storeN with "Hl").
@@ -339,7 +552,7 @@ Lemma wp_length pe E l dq vs :
   {{{ RET LitV $ LitInt (length vs); l ↦∗{dq} vs }}}.
 Proof.
   iIntros (Φ) ">Hl HΦ". iApply wp_lift_atomic_head_step; first done.
-  iIntros (σ1 ns) "(Hσ & Hsteps) !>". iDestruct (gen_heap_valid with "Hσ Hl") as %?.
+  iIntros (σ1 ns) "(Hσ & Hsteps & Hrem) !>". iDestruct (gen_heap_valid with "Hσ Hl") as %?.
   iSplit; first by eauto with head_step.
   iIntros (v2 σ2 Hstep); inv_head_step. iModIntro.
   iMod (steps_auth_update_S with "Hsteps") as "Hsteps".
