theories/ml_toy_lang/melocoton/examples.v
@@ -31,8 +31,10 @@ Lemma prog_correct
 Proof.
   iStartProof. unfold call_inc.
   wp_pures. unfold Z.add.
-  wp_alloc l as "Hl". wp_pures.
-  wp_store. wp_extern.
+
+  wp_alloc l as "Hl", "Hlive".
+  wp_pures. wp_store.
+  wp_extern.
   iModIntro. cbn. iExists 41%Z. iFrame. iIntros "Hl".
   wp_pures. wp_load. iModIntro. done.
 Qed.
